Fixed tagging to include node timestamp in max; added some step-lemmas for the proof

ironfleet/src/Dafny/Distributed/Common/Framework/Performance.s.dfy
@@ -6,13 +6,21 @@ include "../Collections/Seqs.i.dfy"
 module Performance_s {
   import opened Collections__Seqs_i
 
-  datatype PerformanceReport = None | PerformanceReport(instructions: int, pktsDelivered: int)
+  datatype PerformanceReport = PerfNone | PerformanceReport(instructions: int, pktsDelivered: int)
   type PerfReport = PerformanceReport
 
   predicate {:axiom} PerfLe(lhs:PerfReport, rhs:PerfReport)
 
   function {:axiom} PerfMax(prs:seq<PerformanceReport>): PerformanceReport
     ensures forall pr :: pr in prs ==> PerfLe(pr, PerfMax(prs))
+    ensures PerfNone() in prs ==> PerfMax(prs) == PerfNone()
+    ensures prs == []  ==> PerfMax(prs) == PerfNone()
 
-  function {:axiom} PerfAdd(pr1:PerformanceReport, pr2:PerformanceReport) : PerformanceReport
+  function {:axiom} PerfAdd(prs:multiset<PerformanceReport>) : PerformanceReport
+    ensures PerfNone() in prs ==> PerfAdd(prs) == PerfNone()
+
+  function {:axiom} PerfAdd2(pr1:PerformanceReport, pr2:PerformanceReport) : PerformanceReport
+    ensures PerfAdd2(pr1, pr2) == PerfAdd(multiset{pr1, pr2})
+    ensures pr1 == PerfNone ==> PerfAdd2(pr1, pr2) == PerfNone()
+    ensures pr2 == PerfNone ==> PerfAdd2(pr1, pr2) == PerfNone()
 }
