ironfleet/src/Dafny/Distributed/Protocol/Lock/PerformanceProof/PerformanceProof.i.dfy
@@ -1,9 +1,11 @@
 include "../../../Services/Lock/LockTaggedDistributedSystem.i.dfy"
-  include "TaggedGLS.i.dfy"
+include "TaggedGLS.i.dfy"
+include "Definitions.i.dfy"
 
 module PerformanceProof_i {
 import opened LockTaggedDistributedSystem_i
   import opened TaggedGLS_i
+  import opened PerformanceProof__Definitions_i
 
 predicate SingleGLSPerformanceAssumption(tgls:TaggedGLS_State)
 {
@@ -24,6 +26,98 @@ predicate SingleGLSPerformanceGuarantee(gls:TaggedGLS_State)
 predicate GLSPerformanceGuarantee(tglb:seq<TaggedGLS_State>)
 {
   forall tgls :: tgls in tglb ==> SingleGLSPerformanceGuarantee(tgls)
+}
+
+predicate TGLS_Consistency(tgls: TaggedGLS_State)
+{
+  && (forall id :: id in tgls.tls.config <==> id in tgls.tls.t_servers)
+    && (forall id :: id in tgls.tls.t_servers ==> (tgls.tls.t_servers[id].v.config == tgls.tls.config))
+    && (forall i :: 0 <= i < |tgls.tls.config| ==> tgls.tls.t_servers[tgls.tls.config[i]].v.my_index == i)
+}
+
+predicate PerfInvariantLockHeld(tgls: TaggedGLS_State, j:int)
+    requires 0 <= j < |tgls.tls.config|
+    requires TGLS_Consistency(tgls)
+{
+  tgls.tls.t_servers[tgls.tls.config[j]].v.held == true
+    && |tgls.history| == j + 1
+    && tgls.tls.t_servers[tgls.tls.config[j]].v.epoch == |tgls.history|
+
+    &&  (forall id :: id in tgls.tls.t_servers && id != tgls.tls.config[j]
+    ==> tgls.tls.t_servers[id].v.held == false && tgls.tls.t_servers[id].v.epoch < |tgls.history|)
+    
+    && ( forall pkt :: pkt in tgls.tls.t_environment.sentPackets && pkt.dst in tgls.tls.t_servers && pkt.src in tgls.tls.t_servers
+    && pkt.msg.v.Transfer? ==> !(pkt.dst == tgls.tls.config[0]) )
+
+    // All packets have epoch too small, so that no packets can be accepted in the next step
+    && ( forall pkt :: pkt in tgls.tls.t_environment.sentPackets && pkt.msg.v.Transfer? && pkt.dst in tgls.tls.t_servers && pkt.src in tgls.tls.t_servers
+    ==> pkt.msg.v.transfer_epoch <= tgls.tls.t_servers[pkt.dst].v.epoch)
+
+    // All irrelevant packets have zero PerfReport
+    && ( forall pkt :: pkt in tgls.tls.t_environment.sentPackets && !(pkt.src in tgls.tls.t_servers)
+    ==> pkt.msg.pr == PerfNone())
+
+    // The node with the lock has correct PerfReport
+    && tgls.tls.t_servers[tgls.tls.config[j]].pr == PerfBound(j)
+
+    // If there's a packet that grants lock to node j, it's PerfReport must be correct
+    && ( forall pkt :: pkt in tgls.tls.t_environment.sentPackets && pkt.dst == tgls.tls.config[j] && pkt.dst in tgls.tls.t_servers && pkt.src in tgls.tls.t_servers
+    ==> pkt.msg.pr == PerfBound(j) )
+
+    // All nodes beyond j have zero PerfReport
+    && (forall k :: j < k < |tgls.tls.config| ==> tgls.tls.t_servers[tgls.tls.config[k]].pr == PerfNone() )
+
+    // No packets sent to nodes that have my_index higher than j
+    && (forall pkt, k :: j < k < |tgls.tls.config| && pkt in tgls.tls.t_environment.sentPackets && pkt.dst in tgls.tls.t_servers && pkt.dst != tgls.tls.config[k]
+    ==> !(pkt.src in tgls.tls.t_servers)
+    )
+}
+
+lemma NotHostIos_InvLockHeldImpliesInvLockHeld(j:int, s:TaggedGLS_State, s':TaggedGLS_State)
+  requires TGLS_Next(s, s')
+  requires 0 <= j < |s.tls.config|
+  requires TGLS_Consistency(s) && TGLS_Consistency(s')
+
+  // Not a HostIos step
+  requires !s.tls.t_environment.nextStep.LEnvStepHostIos?
+
+  requires PerfInvariantLockHeld(s, j);
+  ensures PerfInvariantLockHeld(s', j);
+{
+}
+
+lemma Grant_not_j_InvLockHeldImpliesInvLockHeld(j:int, s:TaggedGLS_State, s':TaggedGLS_State)
+  requires TGLS_Next(s, s')
+  requires 0 <= j < |s.tls.config|
+  requires TGLS_Consistency(s) && TGLS_Consistency(s')
+  requires SingleGLSPerformanceAssumption(s)
+
+  // A node other than node j taking a grant step
+  requires s.tls.t_environment.nextStep.LEnvStepHostIos?
+  requires s.tls.t_environment.nextStep.actor != s.tls.config[j]
+  requires s.tls.t_environment.nextStep.nodeStep == GrantStep
+
+  requires PerfInvariantLockHeld(s, j);
+  ensures PerfInvariantLockHeld(s', j);
+{
+}
+
+lemma Accept_not_j_InvLockHeldImpliesInvLockHeld(j:int, s:TaggedGLS_State, s':TaggedGLS_State)
+  requires TGLS_Next(s, s')
+  requires 0 <= j < |s.tls.config|
+  requires TGLS_Consistency(s) && TGLS_Consistency(s')
+  requires SingleGLSPerformanceAssumption(s)
+
+  // A node other than node j taking an accept step
+  requires s.tls.t_environment.nextStep.LEnvStepHostIos?
+  requires s.tls.t_environment.nextStep.actor != s.tls.config[j]
+  requires s.tls.t_environment.nextStep.nodeStep == AcceptStep
+
+  requires PerfInvariantLockHeld(s, j);
+  ensures PerfInvariantLockHeld(s', j);
+{
+  var id := s.tls.t_environment.nextStep.actor;
+  assert s.tls.t_servers[id].pr == PerfNone();
 }
 
 lemma PerformanceGuaranteeHolds(config:Config, tglb:seq<TaggedGLS_State>)
