ironfleet/src/Dafny/Distributed/Protocol/Lock/PerformanceProof/Definitions.i.dfy
@@ -1,0 +1,18 @@
+include "../../../Services/Lock/LockTaggedDistributedSystem.i.dfy"
+  include "TaggedGLS.i.dfy"
+
+module PerformanceProof__Definitions_i {
+import opened LockTaggedDistributedSystem_i
+  // import opened TaggedGLS_i
+
+function PerfBound(epoch: int) : PerfReport
+  requires 0 <= epoch
+{
+  if epoch == 0 then
+    PerfNone()
+  else
+    PerfAdd2(GetStepRuntime(GrantStep), PerfBound(epoch - 1))
+}
+
+  
+}
